bedrock2/src/bedrock2/ProgramLogic.v
@@ -11,20 +11,6 @@ Existing Class spec_of.
 (*Definition ct_spec_of (procname:String.string) := list (String.string * (list String.string * list String.string * Syntax.cmd.cmd)) -> Prop.
 Existing Class ct_spec_of.*)
 
-(* not sure where to put these lemmas *)
-Lemma align_trace_cons {T} x xs cont t (H : xs = List.app cont t) : @List.cons T x xs = List.app (cons x cont) t.
-Proof. intros. cbn. congruence. Qed.
-Lemma align_trace_app {T} x xs cont t (H : xs = List.app cont t) : @List.app T x xs = List.app (List.app x cont) t.
-Proof. intros. cbn. subst. rewrite List.app_assoc; trivial. Qed.
-
-Ltac trace_alignment :=
-    repeat match goal with
-      | t := cons _ _ |- _ => subst t
-      end;
-    repeat (eapply align_trace_app
-            || eapply align_trace_cons
-            || exact (eq_refl (List.app nil _))).
-
 Module Import Coercions.
   Import Map.Interface Word.Interface BinInt.
   Coercion Z.of_nat : nat >-> Z.
